\documentclass[a4paper,12pt]{article}

\usepackage{german}

\usepackage{graphicx}

\usepackage{amssymb}

\usepackage{amsfonts}

\usepackage{amsmath}

\usepackage{amsthm}



\pagestyle{empty}



\begin{document}

estimation of spectral norm of the repeated factor that disrupts the convolution structure of the kth term in the expansion of the S matrix

\begin{multline}%include slash notation
\left\|\frac{\slash{p}+m}{p^2-m^2}\right\|_{\text{spec}}=\left\|\frac{\gamma^\alpha p_\alpha+m}{p^2-m^2}\right\|_{\text{spec}}
=\left\|\frac{\gamma^\alpha \lambda_\alpha -i\epsilon \gamma^0 +m}{\lambda^2-m^2 -2i \epsilon \lambda^0 -\epsilon^2}\right\|_{\text{spec}}
\\=\frac{\left\|\gamma^\alpha \lambda_\alpha -i\epsilon \gamma^0 +m\right\|_{\text{spec}}}{\sqrt{(\lambda^2-m^2  -\epsilon^2)^2+4 \epsilon^2 \left(\lambda^0\right)^2}}
=\frac{\epsilon\left\|\gamma^\alpha \frac{\lambda_\alpha}{\epsilon} -i \gamma^0 +\frac{m}{\epsilon}\right\|_{\text{spec}}}{\epsilon^2\sqrt{\left(\left(\frac{\lambda}{\epsilon}\right)^2-\left(\frac{m}{\epsilon}\right)^2  -1\right)^2+4  \left(\frac{\lambda^0}{\epsilon}\right)^2}}
\\\rightarrow^{\epsilon\rightarrow\infty}_{\frac{\lambda}{\epsilon}=\text{const}}\text{overtext...} =\frac{\left\|\gamma^\alpha z_\alpha -i \gamma^0 \right\|_{\text{spec}}}{\epsilon\sqrt{\left(z^2  -1\right)^2+4  \left(z^0\right)^2}}
\end{multline}
now continue to estimate the resulting expression maximizing over z

\begin{multline}
\frac{\left\|\gamma^\alpha z_\alpha -i \gamma^0 \right\|_{\text{spec}}}{\sqrt{\left(z^2  -1\right)^2+4  \left(z^0\right)^2}}
\le \frac{\left\|\gamma^\alpha z_\alpha \right\|_{\text{spec}} +\left\| \gamma^0 \right\|_{\text{spec}}}{\sqrt{\left(z^2  -1\right)^2+4  \left(z^0\right)^2}}
\le \frac{4 \| z\| +1}{\sqrt{\left(z^2  -1\right)^2+4  \left(z^0\right)^2}}
\\= \frac{4 \| z\| +1}{\sqrt{\left(z^2\right)^2  +1+2  \left\|z\right\|^2}}
\le \frac{4 \| z\| +1}{\sqrt{1+2  \left\|z\right\|^2}}\le 2\sqrt{2}
\end{multline}

,where the last estimation follows from analyzing the differentiation of the second but last expression with respect to \(\| z \|\):

\end{document}

